Split code and define basic Makefile

day1/closed.fst
@@ -5,8 +5,8 @@ open Ast
 
 let rec closed l = function
     | Annoted e t -> closed l e
-    | Bound j     -> if List.mem j l then return () else throwError "unbound variable"
-    | Free x      -> return ()
-    | Apply e1 e2 -> closed l e1 >>= (fun _ -> closed l e2)
+    | Bound j     -> List.mem j l
+    | Free x      -> true
+    | Apply e1 e2 -> closed l e1 && closed l e2
     | Inferable e -> closed l e
     | Lambda e    -> closed l e
