day1/utils.fst
@@ -1,3 +1,6 @@
 module Utils
 
+let (<%) f g = fun a -> f (g a)
+let (%>) g f = f <% g
 let constant b _ = b
+let flip f a b = f b a
