day1/closed.fsti
@@ -3,5 +3,5 @@ module Closed
 open Try
 open Ast
 
-val closed : (#a:Type) -> list nat -> e:term a -> Tot (result unit) (decreases e)
+val closed : (#a:Type) -> list nat -> e:term a -> Tot bool // (decreases e)
 
