day1/utils.fsti
@@ -1,3 +1,6 @@
 module Utils
 
-val constant    : (#a:Type) -> (#b :Type) -> b -> a -> Tot b
+val (<%)     : (#a:Type) -> (#b :Type) -> (#c :Type) -> (b -> c) -> (a -> b) -> a -> c
+val (%>)     : (#a:Type) -> (#b :Type) -> (#c :Type) -> (a -> b) -> (b -> c) -> a -> c
+val constant : (#a:Type) -> (#b :Type) -> b -> a -> Tot b
+val flip     : (#a:Type) -> (#b :Type) -> (#c :Type) -> (a -> b -> c) -> (b -> a -> c)
